wip on an ad-hoc interface for HSL

src/tls/HandshakeLogLow.fsti
@@ -142,6 +142,9 @@ val hsl_output_buf : st:hsl_state -> GTot (lbuffer8 (hsl_output_buf_len st))
 val hsl_output_index : HS.mem -> st:hsl_state -> GTot (i:uint_32{i <= hsl_output_buf_len st})
 
 
+val hsl_input_hash_index (h:HS.mem) (st:hsl_state) : GTot uint_32
+
+
 /// HSL footprint
 /// Local footprint is abstract and is allocated in the region provided at the creation time
 
@@ -199,6 +202,7 @@ unfold private let create_post (r:Mem.rgn)
     hsl_output_buf_len st == output_len /\ hsl_output_buf st == output_buf /\  //I/O bufs are as given
     hsl_input_index h1 st == 0ul /\  //input index is 0
     hsl_output_index h1 st == 0ul /\  //output index is 0
+    hsl_input_hash_index h1 st == 0ul /\
     B.fresh_loc (hsl_local_footprint st) h0 h1 /\  //local footprint is fresh
     B.loc_includes (B.loc_regions true (Set.singleton r)) (hsl_local_footprint st) /\  //TODO: local footprint is in r only
     hsl_invariant h1 st /\  //invariant holds
@@ -227,6 +231,7 @@ unfold private let set_params_post (st:hsl_state) (a:Hashing.alg)
     writing h1 st == writing h0 st /\  //writing capability remains same
     hsl_input_index h1 st == hsl_input_index h0 st /\  //input index remains same
     hsl_output_index h1 st == hsl_output_index h0 st /\  //output index remains same
+    hsl_input_hash_index h1 st == hsl_input_hash_index h0 st /\  //output index remains same
     hash_alg h1 st == Some a /\  //hash algorithm is set
     hsl_invariant h1 st  //invariant holds
                          //NB: we are not saying hsl_footprint is same explicitly, it is derivable though, as shown below
@@ -251,304 +256,388 @@ val tags (a:Hash.alg) (prior:list msg) (ms:list msg) (hs:list HashSpec.anyTag) :
 /// Receive returns flight_t with postcondition that the indices are valid parsings in the input buffer
 /// Taken from the match in Handshakre receive function
 
+/// ad-hoc flight types
+/// HS would ask HSL to parse specific flight types, depending on where its state machine is
+
+noeq
+type flight_hrr = {
+  begin_hrr : uint_32;          //begin index in the input buffer
+  hrr_msg   : G.erased HSM.hrr  //erased HelloRetryrequest hrr_msg
+}
+
+noeq
+type flight_c_ske_shd = {
+  begin_c   : uint_32;
+  begin_ske : uint_32;
+  begin_shd : uint_32;
+  c_msg     : G.erased HSM.crt;
+  ske_msg   : G.erased HSM.ske;
+  
+  //no payload in the SHD message
+}
+
+/// AR: other flights would be defined similarly, not defining them since it would change when we use QD types
+
+
+/// LowParse definition of saying buf is a valid serialization of m
+val valid_parsing_aux (m:HSM.hs_msg) (buf:B.buffer uint_8) (h:HS.mem) : Type0
+
+/// Helper to enforce spatial safety of indices in the st input buffer
+unfold let valid_parsing (m:HSM.hs_msg) (begin_idx:uint_32) (end_idx:uint_32) (st:hsl_state) (h:HS.mem) =
+  begin_idx <= end_idx /\ end_idx <= hsl_input_buf_len st /\
+  (let buf = B.gsub (hsl_input_buf st) begin_idx (end_idx - begin_idx) in
+   valid_parsing_aux m buf h)
+
+/// Validitity postcondition on the flights
+
+let valid_flight_hrr (flt:flight_hrr) (flight_end:uint_32) (st:hsl_state) (h:HS.mem) =
+  valid_parsing (HSM.HelloRetryRequest (G.reveal flt.hrr_msg)) flt.begin_hrr flight_end st h
+
+let valid_flight_c_ske_shd (flt:flight_c_ske_shd) (flight_end:uint_32) (st:hsl_state) (h:HS.mem) =
+  (* c msg *)
+  valid_parsing (HSM.Certificate (G.reveal flt.c_msg)) flt.begin_c flt.begin_ske st h /\
+  (* ske msg *)
+  valid_parsing (HSM.ServerKeyExchange (G.reveal flt.ske_msg)) flt.begin_ske flt.begin_shd st h /\
+  (* shd *)
+  valid_parsing HSM.ServerHelloDone flt.begin_shd flight_end st h
+
+(* ... and so on for other flights *)
+
+unfold private let receive_pre (st:hsl_state) (p:uint_32) : HS.mem -> Type0
+  = fun h0 ->
+    hsl_invariant h0 st /\        //invariant should hold
+    hsl_input_index h0 st <= p /\  //should have written >= 0 bytes (> 0?)
+    p <= hsl_input_buf_len st   //p should be in the input buffer range
+
+unfold private let receive_post_basic (st:hsl_state) (p:uint_32) (h0 h1:HS.mem) =
+  B.modifies (hsl_local_footprint st) h0 h1 /\  //only local footprint is modified
+  hash_alg h1 st == hash_alg h0 st /\  //hash alg remains same
+  hsl_invariant h1 st /\  //invariant holds in h1
+  hsl_output_index h1 st == hsl_output_index h0 st /\  //output index remains same
+  hsl_input_index h1 st == p /\  //input index is advanced to p
+  hsl_input_hash_index h1 st == hsl_input_hash_index h0 st /\
+  transcript h0 st == transcript h1 st  //transcript remains same, as it represents the hashed transcript
+
+unfold private let receive_post_common (st:hsl_state) (p:uint_32) (eof:uint_32) (h1:HS.mem) =
+  writing h1 st /\ eof <= p
+
+val receive_flight_hrr (st:hsl_state) (p:uint_32)
+  : ST (TLSError.result (option (flight_hrr &  //returned flight
+                                 uint_32)))    //end input buffer index for the flight
+       (requires (receive_pre st p))
+       (ensures  (fun h0 r h1 ->
+                  let open FStar.Error in
+                  receive_post_basic st p h0 h1 /\  //this is unconditional on parsing success/failure
+		  (match r with
+		   | Error _ -> True  //underspecified
+		   | Correct None -> True  //waiting for more data
+		   | Correct (Some (flt, eof)) ->
+		     valid_flight_hrr flt eof st h1 /\  //flight specific postcondition
+		     receive_post_common st p eof h1)))
+
+val receive_flight_c_ske_shd (st:hsl_state) (p:uint_32)
+  : ST (TLSError.result (option (flight_c_ske_shd &  //returned flight
+                                 uint_32)))          //end input buffer index for the flight
+       (requires (receive_pre st p))
+       (ensures  (fun h0 r h1 ->
+                  let open FStar.Error in
+                  receive_post_basic st p h0 h1 /\  //this is unconditional on parsing success/failure
+		  (match r with
+		   | Error _ -> True  //underspecified
+		   | Correct None -> True  //waiting for more data
+		   | Correct (Some (flt, eof)) ->
+		     valid_flight_c_ske_shd flt eof st h1 /\  //flight specific postcondition
+		     receive_post_common st p eof h1)))
+
+val hash_input (st:hsl_state) (p:uint_32) (
+
+
+// unfold private let receive_post (st:hsl_state) (p:uint_32)
+//   : HS.mem -> (TLSError.result (option (
+//                                flight_t &
+//                                G.erased (list msg) &
+//                                uint_32 & uint_32))) -> HS.mem -> Type0
+//   = fun h0 r h1 ->  
+//     let open FStar.Error in
+//     let oa = hash_alg h0 st in
+//     let t0 = transcript h0 st in
+//     let t1 = transcript h1 st in
+//     (match r with
+//      | Error _ -> True  //underspecified
+//      | Correct None -> t0 == t1  //waiting for more data
+//      | Correct (Some (flt, ms, p0, p1, hs)) ->
+//        let ms = G.reveal ms in
+//        t1 == t0 @ ms /\  //added ms to the transcript
+//        writing h1 st /\  //Handshake can now write
+//        p <= hsl_input_buf_len st /\
+//        p0 <= p1 /\ p1 <= p /\  //returned indices are valid in the input buffer
+//        msg_list_parsing_of ms st p0 p1 h1 /\  //ms is a valid parsing of input buffer contents between p0 and p1
+//        flight_parsing_of flt ms st h1 /\  //the indices in the returned flight are valid parsings
+//        (match oa with
+//         | Some a -> tags a t0 ms hs  //hashed properly
+//         | None -> hs == []))
+
+
+
+
+
 (*
  * CF: make these fine grained, in collaboration with HS
  *)
-type flight_t =
-  | F_HRR: init:uint_32 -> len:uint_32 -> flight_t
-  | F_SH: init:uint_32 -> len:uint_32 -> flight_t
-  | F_C_SKE_SHD: c_init:uint_32 -> c_len:uint_32 ->
-                 ske_init:uint_32 -> ske_len:uint_32 -> 
-		 -> erased certificate -> erased ske ->
-		 flight_t
-  | F_C_SKE_CR_SHD: c_init:uint_32 -> c_len:uint_32 ->
-                    ske_init:uint_32 -> ske_len:uint_32 ->
-                    cr_init:uint_32 -> cr_len:uint_32 -> flight_t
-  | F_EE_C13_CV_Fin: ee_init:uint_32 ->
-                     c13_init:uint_32 ->
-		     cv_init:uint_32 ->
-		     fin_init:uint_32 -> fin_len:uint_32 -> flight_t
-  | F_EE_CR13_C13_CV_Fin: ee_init:uint_32 -> ee_len:uint_32 ->
-                          cr13_init:uint_32 -> cr13_len:uint_32 ->
-			  c13_init:uint_32 -> c13_len:uint_32 ->
-			  cv_init:uint_32 -> cv_len:uint_32 ->
-			  fin_init:uint_32 -> fin_len:uint_32 -> flight_t
-  | F_EE_Fin: ee_init:uint_32 -> ee_len:uint_32 ->
-              fin_init:uint_32 -> fin_len:uint_32 -> flight_t
-  | F_Fin: fin_init:uint_32 -> fin_len:uint_32 -> flight_t
-  | F_CH: ch_init:uint_32 -> ch_len:uint_32 -> flight_t
-  | F_CH_Bind: ch_init:uint_32 -> ch_len:uint_32 ->
-               bind_init:uint_32 -> bind_len:uint_32 -> flight_t
-  | F_C13_CV_Fin: c13_init:uint_32 -> c13_len:uint_32 ->
-                  cv_init:uint_32 -> cv_len:uint_32 ->
-		  fin_init:uint_32 -> fin_len:uint_32 -> flight_t
-  | F_EoED: flight_t
-  | F_NST13: nst13_init:uint_32 -> nst13_len:uint_32 -> flight_t
+// type flight_t =
+//   | F_HRR: init:uint_32 -> len:uint_32 -> flight_t
+//   | F_SH: init:uint_32 -> len:uint_32 -> flight_t
+//   | F_C_SKE_SHD: c_init:uint_32 -> c_len:uint_32 ->
+//                  ske_init:uint_32 -> ske_len:uint_32 -> 
+// 		 -> erased certificate -> erased ske ->
+// 		 flight_t
+//   | F_C_SKE_CR_SHD: c_init:uint_32 -> c_len:uint_32 ->
+//                     ske_init:uint_32 -> ske_len:uint_32 ->
+//                     cr_init:uint_32 -> cr_len:uint_32 -> flight_t
+//   | F_EE_C13_CV_Fin: ee_init:uint_32 ->
+//                      c13_init:uint_32 ->
+// 		     cv_init:uint_32 ->
+// 		     fin_init:uint_32 -> fin_len:uint_32 -> flight_t
+//   | F_EE_CR13_C13_CV_Fin: ee_init:uint_32 -> ee_len:uint_32 ->
+//                           cr13_init:uint_32 -> cr13_len:uint_32 ->
+// 			  c13_init:uint_32 -> c13_len:uint_32 ->
+// 			  cv_init:uint_32 -> cv_len:uint_32 ->
+// 			  fin_init:uint_32 -> fin_len:uint_32 -> flight_t
+//   | F_EE_Fin: ee_init:uint_32 -> ee_len:uint_32 ->
+//               fin_init:uint_32 -> fin_len:uint_32 -> flight_t
+//   | F_Fin: fin_init:uint_32 -> fin_len:uint_32 -> flight_t
+//   | F_CH: ch_init:uint_32 -> ch_len:uint_32 -> flight_t
+//   | F_CH_Bind: ch_init:uint_32 -> ch_len:uint_32 ->
+//                bind_init:uint_32 -> bind_len:uint_32 -> flight_t
+//   | F_C13_CV_Fin: c13_init:uint_32 -> c13_len:uint_32 ->
+//                   cv_init:uint_32 -> cv_len:uint_32 ->
+// 		  fin_init:uint_32 -> fin_len:uint_32 -> flight_t
+//   | F_EoED: flight_t
+//   | F_NST13: nst13_init:uint_32 -> nst13_len:uint_32 -> flight_t
 
 
-/// Current flight that has been dispatched to Handshake but is in the process of being hashed
+// /// Current flight that has been dispatched to Handshake but is in the process of being hashed
 
-val current_flight (st:hsl_state) (h:HS.mem) : GTot flight_t
-
-
-type flgithval current_hash_index (st:hsl_state) (h:HS.mem) : GTot uint_32
-
-/// Framing of current flight, current flight index w.r.t. modifications to local state
+// val current_flight (st:hsl_state) (h:HS.mem) : GTot flight_t
 
 
-let is_valid_hash_index (st:hsl_state) (i:uint_32) (h:HS.mem) : GTot bool =
-  let flt = current_flight st h in
-  match flt with
-  | F_HRR init len -> i == init + len
-  | _ -> admit ()
+// type flgithval current_hash_index (st:hsl_state) (h:HS.mem) : GTot uint_32
 
-let end_of_flight_index (st:hsl_state) (h:HS.memt) : GTot uint_32 =
-  let flt = current_flight st h in
-  match flt with
-  | F_HRR init len -> init + len
-  | _ -> admit ()
+// /// Framing of current flight, current flight index w.r.t. modifications to local state
 
 
-/// Do we need to provide 
+// let is_valid_hash_index (st:hsl_state) (i:uint_32) (h:HS.mem) : GTot bool =
+//   let flt = current_flight st h in
+//   match flt with
+//   | F_HRR init len -> i == init + len
+//   | _ -> admit ()
 
-(*
- * Separate into two: one that computes hash and one that returns it
- * Transcript should reflect partial flights that have been hashed
- * Additional state in HSL to maintain this
- *)
-val hash (st:hsl_state) (i:uint_32)
-  : ST unit (requires (fun h0 -> is_valid_hash_index st i /\ i > current_hash_index st h))
-            (ensures  (fun h0 _ h1 -> current_hash_index st h1 == i /\ modifies (hsl_local_footprint st) h0 h1 /\
-	               i == end_of_flight_index st h0 ==>
-		         (writing h1 st /\
-			  transcript h1 st == transcript h0 st @ current_hs_flight st h0)))
+// let end_of_flight_index (st:hsl_state) (h:HS.memt) : GTot uint_32 =
+//   let flt = current_flight st h in
+//   match flt with
+//   | F_HRR init len -> init + len
+//   | _ -> admit ()
 
 
+// /// Do we need to provide 
 
-Option a.
-
-HSL doesn't care what you hash on the receive side.
-HS maintains enough invariants to make sure
-it has hashed the input messages using the ghost messages HSL.receive returned.
-HS maintains the postcondition that transcript has increased when it calls HSL.hash
-Generic precondition of calling HSL.hash
-
-Pros: helps with binders, can hash in the middle of messages
-
-Cons: writing capability maintenance moves to HS for the input flight hashing part, except when HSL is in the middle of reading a flight, HSL switches to writing when it has received a flight
-
-hash (i:uint_32) (j:uint_32)
-     (msgs:erased (list msgs){msgs is parsing of input buffer from i to j})
-     (* can we make it so that it is not erased (list (erased msg)) *)
-  : ensures (transcript is appended to by msgs)
+// (*
+//  * Separate into two: one that computes hash and one that returns it
+//  * Transcript should reflect partial flights that have been hashed
+//  * Additional state in HSL to maintain this
+//  *)
+// val hash (st:hsl_state) (i:uint_32)
+//   : ST unit (requires (fun h0 -> is_valid_hash_index st i /\ i > current_hash_index st h))
+//             (ensures  (fun h0 _ h1 -> current_hash_index st h1 == i /\ modifies (hsl_local_footprint st) h0 h1 /\
+// 	               i == end_of_flight_index st h0 ==>
+// 		         (writing h1 st /\
+// 			  transcript h1 st == transcript h0 st @ current_hs_flight st h0)))
 
 
-On the writing side, it is the same--hashing is done by HSL when HS calls HSL.send
 
-send (...)
-  : ensures (transcript is extedned automatically)
+// // Option a.
+
+// // HSL doesn't care what you hash on the receive side.
+// // HS maintains enough invariants to make sure
+// // it has hashed the input messages using the ghost messages HSL.receive returned.
+// // HS maintains the postcondition that transcript has increased when it calls HSL.hash
+// // Generic precondition of calling HSL.hash
+
+// // Pros: helps with binders, can hash in the middle of messages
+
+// // Cons: writing capability maintenance moves to HS for the input flight hashing part, except when HSL is in the middle of reading a flight, HSL switches to writing when it has received a flight
+
+// // hash (i:uint_32) (j:uint_32)
+// //      (msgs:erased (list msgs){msgs is parsing of input buffer from i to j})
+// //      (* can we make it so that it is not erased (list (erased msg)) *)
+// //   : ensures (transcript is appended to by msgs)
 
 
--- State of hash
--- State of incoming flight, what we are trying to receive
--- Internal state of HSL is like a tree what all flights can we receive
--- Precondition of receive depending on the states
-   Next kind of flight? Should HSL keep track of it?
--- No flight_t and having ad-hoc receive messages
+// // On the writing side, it is the same--hashing is done by HSL when HS calls HSL.send
+
+// // send (...)
+// //   : ensures (transcript is extedned automatically)
 
 
-Whatever we send is a valid receive flight at the other end?
-Peer state machine will accept what we send
+// // -- State of hash
+// // -- State of incoming flight, what we are trying to receive
+// // -- Internal state of HSL is like a tree what all flights can we receive
+// // -- Precondition of receive depending on the states
+// //    Next kind of flight? Should HSL keep track of it?
+// // -- No flight_t and having ad-hoc receive messages
 
-#reset-options "--max_fuel 0 --initial_ifuel 1 --max_ifuel 1"
 
-/// TODO: should come from QD
+// // Whatever we send is a valid receive flight at the other end?
+// // Peer state machine will accept what we send
 
-type parser_t (a:Type) = LP.parser (LP.strong_parser_kind 8 8 ({ LP.parser_kind_metadata_total = true })) a
+// #reset-options "--max_fuel 0 --initial_ifuel 1 --max_ifuel 1"
 
-val hrr_parser : parser_t HSM.hrr
-val sh_parser : parser_t HSM.sh
-val c_parser : parser_t HSM.crt
-val ske_parser : parser_t HSM.ske
-val cr_parser : parser_t HSM.cr
+// /// TODO: should come from QD
 
-unfold let valid_parsing (#a:Type) (m:a) (parser:parser_t a) (buf:B.buffer uint_8) (h:HS.mem) =
-  match LP.parse parser (B.as_seq h buf) with
-  | None -> False
-  | Some (parse, consumed) -> parse == m /\ consumed == B.length buf
 
-unfold let valid_init_and_len (init len:uint_32) (st:hsl_state) =
-  init <= len /\ within_bounds (Unsigned W32) (v init + v len) /\ init + len <= hsl_input_buf_len st  
+// val hrr_parser : parser_t HSM.hrr
+// val sh_parser : parser_t HSM.sh
+// val c_parser : parser_t HSM.crt
+// val ske_parser : parser_t HSM.ske
+// val cr_parser : parser_t HSM.cr
 
-/// Predicate for flight being a valid parsing
-/// In addition to this, the postcondition of receive also establishes valid parsing of the transcript itself
+// unfold let valid_parsing (#a:Type) (m:a) (parser:parser_t a) (buf:B.buffer uint_8) (h:HS.mem) =
+//   match LP.parse parser (B.as_seq h buf) with
+//   | None -> False
+//   | Some (parse, consumed) -> parse == m /\ consumed == B.length buf
 
-let flight_parsing_of (flt:flight_t) (msgs:hs_transcript) (st:hsl_state) (h:HS.mem) =
-  match flt with
-  | F_HRR init len ->
-    valid_init_and_len init len st /\
-    (match msgs with
-     | [ HSM.HelloRetryRequest r ] -> valid_parsing r hrr_parser (B.gsub (hsl_input_buf st) init len) h
-     | _ -> False)
+// unfold let valid_init_and_len (init len:uint_32) (st:hsl_state) =
+//   init <= len /\ within_bounds (Unsigned W32) (v init + v len) /\ init + len <= hsl_input_buf_len st  
 
-  | F_SH init len ->
-    valid_init_and_len init len st /\
-    (match msgs with
-     | [ HSM.ServerHello sh ] -> valid_parsing sh sh_parser (B.gsub (hsl_input_buf st) init len) h
-     | _ -> False)
+// /// Predicate for flight being a valid parsing
+// /// In addition to this, the postcondition of receive also establishes valid parsing of the transcript itself
 
-  | F_C_SKE_SHD c_init ske_init ske_len ->
-    valid_init_and_len c_init c_len st /\ valid_init_and_len ske_init ske_len st /\
-    (match msgs with
-     | [ HSM.Certificate c; HSM.ServerKeyExchange ske; HSM.ServerHelloDone ] ->
-       valid_parsing c c_parser (B.gsub (hsl_input_buf st) c_init c_len) h /\
-       valid_parsing ske ske_parser (B.gsub (hsl_input_buf st) ske_init ske_len) h
-     | _ -> False)
+// let flight_parsing_of (flt:flight_t) (msgs:hs_transcript) (st:hsl_state) (h:HS.mem) =
+//   match flt with
+//   | F_HRR init len ->
+//     valid_init_and_len init len st /\
+//     (match msgs with
+//      | [ HSM.HelloRetryRequest r ] -> valid_parsing r hrr_parser (B.gsub (hsl_input_buf st) init len) h
+//      | _ -> False)
 
-  | F_C_SKE_CR_SHD c_init c_len ske_init ske_len cr_init cr_len ->
-    valid_init_and_len c_init c_len st /\ valid_init_and_len ske_init ske_len st /\ valid_init_and_len cr_init cr_len st /\
-    (match msgs with
-     | [ HSM.Certificate c; HSM.ServerKeyExchange ske; HSM.CertificateRequest cr; HSM.ServerHelloDone ] ->
-       valid_parsing c c_parser (B.gsub (hsl_input_buf st) c_init c_len) h /\
-       valid_parsing ske ske_parser (B.gsub (hsl_input_buf st) ske_init ske_len) h /\
-       valid_parsing cr cr_parser (B.gsub (hsl_input_buf st) cr_init cr_len) h
-     | _ -> False)
+//   | F_SH init len ->
+//     valid_init_and_len init len st /\
+//     (match msgs with
+//      | [ HSM.ServerHello sh ] -> valid_parsing sh sh_parser (B.gsub (hsl_input_buf st) init len) h
+//      | _ -> False)
 
-  //TODO: fill other entries similarly
+//   | F_C_SKE_SHD c_init ske_init ske_len ->
+//     valid_init_and_len c_init c_len st /\ valid_init_and_len ske_init ske_len st /\
+//     (match msgs with
+//      | [ HSM.Certificate c; HSM.ServerKeyExchange ske; HSM.ServerHelloDone ] ->
+//        valid_parsing c c_parser (B.gsub (hsl_input_buf st) c_init c_len) h /\
+//        valid_parsing ske ske_parser (B.gsub (hsl_input_buf st) ske_init ske_len) h
+//      | _ -> False)
 
-  | _ -> False
+//   | F_C_SKE_CR_SHD c_init c_len ske_init ske_len cr_init cr_len ->
+//     valid_init_and_len c_init c_len st /\ valid_init_and_len ske_init ske_len st /\ valid_init_and_len cr_init cr_len st /\
+//     (match msgs with
+//      | [ HSM.Certificate c; HSM.ServerKeyExchange ske; HSM.CertificateRequest cr; HSM.ServerHelloDone ] ->
+//        valid_parsing c c_parser (B.gsub (hsl_input_buf st) c_init c_len) h /\
+//        valid_parsing ske ske_parser (B.gsub (hsl_input_buf st) ske_init ske_len) h /\
+//        valid_parsing cr cr_parser (B.gsub (hsl_input_buf st) cr_init cr_len) h
+//      | _ -> False)
+
+//   //TODO: fill other entries similarly
+
+//   | _ -> False
        
   
-/// TODO: Should come from QD
+// /// TODO: Should come from QD
 
-val hs_transcript_parser : LP.parser (LP.strong_parser_kind 8 8 ({ LP.parser_kind_metadata_total = true })) hs_transcript
+// val hs_transcript_parser : LP.parser (LP.strong_parser_kind 8 8 ({ LP.parser_kind_metadata_total = true })) hs_transcript
 
-(* msgs is parsing of the input sub-buffer between p0 and p1 *)
-unfold private let msg_list_parsing_of (msgs:hs_transcript) (st:hsl_state)
-                                       (p0:uint_32) (p1:uint_32{p0 <= p1 /\ p1 <= hsl_input_buf_len st})
-			               (h:HS.mem)
-  = let delta = p1 - p0 in
-    let sub = B.gsub (hsl_input_buf st) p0 delta in
-    match LP.parse hs_transcript_parser (B.as_seq h sub) with
-    | None -> False
-    | Some (parse, consumed) -> parse == msgs /\ consumed == v delta
+// (* msgs is parsing of the input sub-buffer between p0 and p1 *)
+// unfold private let msg_list_parsing_of (msgs:hs_transcript) (st:hsl_state)
+//                                        (p0:uint_32) (p1:uint_32{p0 <= p1 /\ p1 <= hsl_input_buf_len st})
+// 			               (h:HS.mem)
+//   = let delta = p1 - p0 in
+//     let sub = B.gsub (hsl_input_buf st) p0 delta in
+//     match LP.parse hs_transcript_parser (B.as_seq h sub) with
+//     | None -> False
+//     | Some (parse, consumed) -> parse == msgs /\ consumed == v delta
 
-(*
- * CF: Remember indices in the input buffer for transcripts
- *     May be just keep index until t0
- *     For incremental hashing for t1, keep states in between
- *     Hashing can be part of the state
- *     After delivering the flight, and before starting new flight,
- *       remember where is hashing state (index)
- *     Also hashing state is just Evercrypt hash state
- *     Return hash value on the caller stack
- *     Transcript is the hashed transcript? Add messages to transcrip
- *       when hashed after call to HS
- *     HSLog maintains hashed transcript
- *       and indices for the last flight returned -- so that it can relate Hash calls from HS
- *)
+// (*
+//  * CF: Remember indices in the input buffer for transcripts
+//  *     May be just keep index until t0
+//  *     For incremental hashing for t1, keep states in between
+//  *     Hashing can be part of the state
+//  *     After delivering the flight, and before starting new flight,
+//  *       remember where is hashing state (index)
+//  *     Also hashing state is just Evercrypt hash state
+//  *     Return hash value on the caller stack
+//  *     Transcript is the hashed transcript? Add messages to transcrip
+//  *       when hashed after call to HS
+//  *     HSLog maintains hashed transcript
+//  *       and indices for the last flight returned -- so that it can relate Hash calls from HS
+//  *)
 
-(* pair of ints can be computed from flight_t *)
-(* flight_t with indices and erased messages with postconditions for relating them *)
-
-unfold private let receive_post (st:hsl_state) (p:uint_32)
-  : HS.mem -> (TLSError.result (option (
-                               flight_t &
-                               G.erased (list msg) &
-                               uint_32 & uint_32))) -> HS.mem -> Type0
-  = fun h0 r h1 ->  
-    let open FStar.Error in
-    let oa = hash_alg h0 st in
-    let t0 = transcript h0 st in
-    let t1 = transcript h1 st in
-    B.modifies (hsl_local_footprint st) h0 h1 /\  //only local footprint is modified
-    hash_alg h1 st == oa /\  //hash alg remains same
-    hsl_invariant h1 st /\  //invariant holds
-    hsl_output_index h1 st == hsl_output_index h0 st /\  //output index remains same
-    hsl_input_index h1 st == p /\  //input index is advanced to p
-    t0 == t1 /\  //transcript remains same, as it represents the hashed transcript
-    (match r with
-     | Error _ -> True  //underspecified
-     | Correct None -> t0 == t1  //waiting for more data
-     | Correct (Some (flt, ms, p0, p1, hs)) ->
-       let ms = G.reveal ms in
-       t1 == t0 @ ms /\  //added ms to the transcript
-       writing h1 st /\  //Handshake can now write
-       p <= hsl_input_buf_len st /\
-       p0 <= p1 /\ p1 <= p /\  //returned indices are valid in the input buffer
-       msg_list_parsing_of ms st p0 p1 h1 /\  //ms is a valid parsing of input buffer contents between p0 and p1
-       flight_parsing_of flt ms st h1 /\  //the indices in the returned flight are valid parsings
-       (match oa with
-        | Some a -> tags a t0 ms hs  //hashed properly
-        | None -> hs == []))
-
-//TODO: delay the hashing OR Handshake explicitly calls Log to compute the digest 
-val receive (st:hsl_state) (p:uint_32)
-  : ST (TLSError.result (option (flight_t &  //returned flight
-                                 G.erased hs_transcript &  //ghost transcript, list msg or hs_transcript
-                                 uint_32 & uint_32 &  //buffer indices in the input buffer
-                                 list HashSpec.anyTag)))  //TODO: erased transcript and concrete hash?
-       (requires (fun h0 ->
-                  hsl_invariant h0 st /\  //invariant should hold
-                  hsl_input_index h0 st <= p /\  //TODO: should have written >= 0 bytes (> 0?)
-		  p <= hsl_input_buf_len st))  //p should be in the input buffer range
-       (ensures  (receive_post st p))
+// (* pair of ints can be computed from flight_t *)
+// (* flight_t with indices and erased messages with postconditions for relating them *)
 
 
-/// TODO: receive_CCS
+// //TODO: delay the hashing OR Handshake explicitly calls Log to compute the digest 
 
 
-/// Send API
+// /// TODO: receive_CCS
 
-/// TODO: should come from QD
 
-val msg_parser : parser_t msg
+// /// Send API
 
-unfold private let msg_parsing_of (m:msg) (st:hsl_state)
-                                  (p0:uint_32) (p1:uint_32{p0 <= p1 /\ p1 <= hsl_output_buf_len st})
-			          (h:HS.mem)
-  = let delta = p1 - p0 in
-    let sub = B.gsub (hsl_output_buf st) p0 delta in
-    match LP.parse msg_parser (B.as_seq h sub) with
-    | None -> False
-    | Some (parse, consumed) -> parse == m /\ consumed == v delta
+// /// TODO: should come from QD
 
-unfold private let send_pre (st:hsl_state) (p:uint_32) (m:G.erased msg)
-  : HS.mem -> Type0
-  = fun h0 ->
-    let open HandshakeMessages in
-    hsl_invariant h0 st /\  //invariant holds
-    hsl_output_index h0 st <= p /\ p <= hsl_output_buf_len st /\  //p is in range of output buffer
-    msg_parsing_of (G.reveal m) st (hsl_output_index h0 st) p h0 /\  //m is a valid parsing of sub-buffer between p0 and p1
-    writing h0 st /\  //Handshake is allowed to write
-    valid_transcript (transcript h0 st @ [G.reveal m]) /\  //valid transcript
-    (match G.reveal m with  //copied from HandshakeLog as is
-     | HelloRetryRequest req -> Some? (C.cipherSuite_of_name req.hrr_cipher_suite)
-     | _ -> True)
+// val msg_parser : parser_t msg
 
-unfold private let send_post (st:hsl_state) (p:uint_32) (m:G.erased msg)
-  : HS.mem -> unit -> HS.mem -> Type0
-  = fun h0 _ h1 ->
-    B.modifies (hsl_local_footprint st) h0 h1 /\  //only local footprint is modified
-    writing h1 st /\  //writing capability remains
-    hash_alg h1 st == hash_alg h0 st /\  //hash algorithm is same as before
-    transcript h1 st == transcript h0 st @ [G.reveal m] /\  //transcript includes m
-    hsl_invariant h1 st /\  //invariant hold
-    hsl_input_index h1 st == hsl_input_index h0 st /\  //input buffer index remains same
-    hsl_output_index h1 st == p  //output buffer index is advanced to p
+// unfold private let msg_parsing_of (m:msg) (st:hsl_state)
+//                                   (p0:uint_32) (p1:uint_32{p0 <= p1 /\ p1 <= hsl_output_buf_len st})
+// 			          (h:HS.mem)
+//   = let delta = p1 - p0 in
+//     let sub = B.gsub (hsl_output_buf st) p0 delta in
+//     match LP.parse msg_parser (B.as_seq h sub) with
+//     | None -> False
+//     | Some (parse, consumed) -> parse == m /\ consumed == v delta
 
-val send (st:hsl_state) (p:uint_32) (m:G.erased msg)
-  : ST unit (requires (send_pre st p m))
-            (ensures  (send_post st p m))
+// unfold private let send_pre (st:hsl_state) (p:uint_32) (m:G.erased msg)
+//   : HS.mem -> Type0
+//   = fun h0 ->
+//     let open HandshakeMessages in
+//     hsl_invariant h0 st /\  //invariant holds
+//     hsl_output_index h0 st <= p /\ p <= hsl_output_buf_len st /\  //p is in range of output buffer
+//     msg_parsing_of (G.reveal m) st (hsl_output_index h0 st) p h0 /\  //m is a valid parsing of sub-buffer between p0 and p1
+//     writing h0 st /\  //Handshake is allowed to write
+//     valid_transcript (transcript h0 st @ [G.reveal m]) /\  //valid transcript
+//     (match G.reveal m with  //copied from HandshakeLog as is
+//      | HelloRetryRequest req -> Some? (C.cipherSuite_of_name req.hrr_cipher_suite)
+//      | _ -> True)
+
+// unfold private let send_post (st:hsl_state) (p:uint_32) (m:G.erased msg)
+//   : HS.mem -> unit -> HS.mem -> Type0
+//   = fun h0 _ h1 ->
+//     B.modifies (hsl_local_footprint st) h0 h1 /\  //only local footprint is modified
+//     writing h1 st /\  //writing capability remains
+//     hash_alg h1 st == hash_alg h0 st /\  //hash algorithm is same as before
+//     transcript h1 st == transcript h0 st @ [G.reveal m] /\  //transcript includes m
+//     hsl_invariant h1 st /\  //invariant hold
+//     hsl_input_index h1 st == hsl_input_index h0 st /\  //input buffer index remains same
+//     hsl_output_index h1 st == p  //output buffer index is advanced to p
+
+// val send (st:hsl_state) (p:uint_32) (m:G.erased msg)
+//   : ST unit (requires (send_pre st p m))
+//             (ensures  (send_post st p m))
 		       
-/// hash_tag API
+// /// hash_tag API
 
-/// TODO: the postcondition fails to typecheck
+// /// TODO: the postcondition fails to typecheck
 
-#push-options "--admit_smt_queries true"
-val hash_tag (a:Hash.alg) (st:hsl_state)
-  : ST (Hash.tag a) (requires (fun h0 -> hsl_invariant h0 st))
-                    (ensures  (fun h0 r h1 ->
-		               let bs = transcript_bytes (transcript h1 st) in
-			       h0 == h1 /\ Hashing.CRF.hashed a bs /\ r == Hash.h a bs))
-#pop-options
+// #push-options "--admit_smt_queries true"
+// val hash_tag (a:Hash.alg) (st:hsl_state)
+//   : ST (Hash.tag a) (requires (fun h0 -> hsl_invariant h0 st))
+//                     (ensures  (fun h0 r h1 ->
+// 		               let bs = transcript_bytes (transcript h1 st) in
+// 			       h0 == h1 /\ Hashing.CRF.hashed a bs /\ r == Hash.h a bs))
+// #pop-options
